src/Lean/Elab/Tactic/Do/ProofMode/Pure.lean
@@ -12,18 +12,19 @@ namespace Lean.Elab.Tactic.Do.ProofMode
 open Std.Do SPred.Tactic
 open Lean Elab Tactic Meta
 
--- NB: We do not use MVarId.intro because that would mean we require all callers to supply an MVarId.
+variable {m : Type → Type u} [Monad m] [MonadControlT MetaM m] [MonadLiftT MetaM m]
+
 -- This function only knows about the hypothesis H=⌜φ⌝ to destruct.
 -- It will provide a proof for Q ∧ H ⊢ₛ T
 -- if `k` produces a proof for Q ⊢ₛ T that may range over a pure proof h : φ.
 -- It calls `k` with the φ in H = ⌜φ⌝ and a proof `h : φ` thereof.
 def mPureCore (σs : Expr) (hyp : Expr) (name : TSyntax ``binderIdent)
-  (k : Expr /-φ:Prop-/ → Expr /-h:φ-/ → MetaM (α × MGoal × Expr)) : MetaM (α × MGoal × Expr) := do
+  (k : Expr /-φ:Prop-/ → Expr /-h:φ-/ → m (α × MGoal × Expr)) : m (α × MGoal × Expr) := do
   let φ ← mkFreshExprMVar (mkSort .zero)
   let inst ← synthInstance (mkApp3 (mkConst ``IsPure) σs hyp φ)
-  let (name, ref) ← getFreshHypName name
+  let (name, ref) ← liftMetaM <| getFreshHypName name
   withLocalDeclD name φ fun h => do
-    addLocalVarInfo ref (← getLCtx) h φ
+    addLocalVarInfo ref (← liftMetaM <| getLCtx) h φ
     let (a, goal, prf /- : goal.toExpr -/) ← k φ h
     let prf ← mkLambdaFVars #[h] prf
     let prf := mkApp7 (mkConst ``Pure.thm) σs goal.hyps hyp goal.target φ inst prf
