src/Lean/Elab/Tactic/Do/ProofMode/Revert.lean
@@ -12,26 +12,120 @@ namespace Lean.Elab.Tactic.Do.ProofMode
 open Std.Do SPred.Tactic
 open Lean Elab Tactic Meta
 
-partial def mRevertStep (goal : MGoal) (ref : TSyntax `ident) (k : MGoal → MetaM Expr) : MetaM Expr := do
+variable {m : Type → Type u} [Monad m] [MonadControlT MetaM m] [MonadLiftT MetaM m]
+
+partial def mRevert (goal : MGoal) (ref : TSyntax `ident) (k : MGoal → m (α × Expr)) : m (α × Expr) := do
   let res ← goal.focusHypWithInfo ref
   let P := goal.hyps
   let Q := res.restHyps
   let H := res.focusHyp
   let T := goal.target
-  let prf ← k { goal with hyps := Q, target := mkApp3 (mkConst ``SPred.imp) goal.σs H T }
+  let (a, prf) ← k { goal with hyps := Q, target := mkApp3 (mkConst ``SPred.imp) goal.σs H T }
   let prf := mkApp7 (mkConst ``Revert.revert) goal.σs P Q H T res.proof prf
-  return prf
+  return (a, prf)
+
+theorem revert_forall_n {α : Type} (H : SPred σs) (T : α → SPred σs) {e₁ : α} (h : H ⊢ₛ T e₁) :
+    SPred.entails (σs:=α::σs) spred((fun s₁ => H) ∧ (fun s₁ => ⌜s₁ = e₁⌝)) T := by
+  intro s
+  mintro h
+  dsimp only [SPred.and_cons]
+  mcases h with ⟨_, ⌜heq⌝⟩
+  subst heq
+  exact h
+
+theorem revert_forall {α : Type} (H : SPred σs) (T : α → SPred σs) {e₁ : α} (h : SPred.entails (σs:=α::σs) spred((fun s₁ => H) ∧ (fun s₁ => ⌜s₁ = e₁⌝)) T) :
+    H ⊢ₛ T e₁ :=
+  Revert.and_pure_intro_r rfl .rfl (h e₁)
+
+theorem revert_forall_2 {α β : Type} (H : SPred σs) (T : α → β → SPred σs) {e₁ : α} {e₂ : β} (h : SPred.entails (σs:=α::β::σs) spred((fun s₁ s₂ => H) ∧ (fun s₁ s₂ => ⌜s₁ = e₁ ∧ s₂ = e₂⌝)) T) :
+    H ⊢ₛ T e₁ e₂ :=
+  --@Revert.and_pure_intro_r σs (e₁ = e₁ ∧ e₂ = e₂) H (T e₁ e₂) ⟨rfl, rfl⟩ (h e₁ e₂)
+  Revert.and_pure_intro_r ⟨rfl, rfl⟩ .rfl (h e₁ e₂)
+
+def mkStateTuple (σs : Expr) : Expr := mkApp (mkConst ``SVal.StateTuple) σs
+def mkSPred (σs : Expr) : Expr := mkApp (mkConst ``SPred) σs
+def mkPureSPred (σs : Expr) (fn : Expr) : Expr :=
+  mkApp3 (mkConst ``SVal.curry) (mkSort 0) σs fn
+def mkAndIntroN (prfs : List Expr) : MetaM Expr := match prfs with
+  | [] => return mkConst ``True.intro
+  | [p] => return p
+  | p::prfs => do mkAppM ``And.intro #[p, ← mkAndIntroN prfs]
+
+/--
+Turn goal
+  hᵢ : Hᵢ
+  ⊢ₛ T e₁ ... eₙ
+into
+  hᵢ : fun sₙ ... s₁ => Hᵢ
+  h : fun sₙ ... s₁ => ⌜s₁ = e₁ ∧ ... ∧ sₙ = eₙ⌝
+  ⊢ₛ T
+-/
+partial def mRevertForallN (goal : MGoal) (n : Nat) (hypName : Name) (k : MGoal → m (α × Expr)) : m (α × Expr) := do
+  if n = 0 then return ← k goal
+  let H := goal.hyps
+  let T := goal.target.consumeMData
+  let f := T.getAppFn
+  let args := T.getAppRevArgs
+  let revertArgs := args[0:n].toArray.reverse
+  unless revertArgs.size = n do
+    liftMetaM <| throwError "mrevert: expected {n} excess arguments in {T}, got {revertArgs.size}"
+  let revertArgsTypes ← liftMetaM <| revertArgs.mapM inferType
+
+  let declInfos ← revertArgsTypes.mapIdxM fun i ty => do
+    return ((← liftMetaM <| mkFreshUserName `s).appendIndexAfter (i+1), ty)
+
+  -- Build `fun s₁ ... sₙ => H ∧ ⌜s₁ = e₁ ∧ ... ∧ sₙ = eₙ⌝`
+  let (H, φ) ← withLocalDeclsDND declInfos fun ss => do
+    let eqs ← (revertArgs.zip ss).mapM fun (e, s) => mkEq s e
+    let eqs := eqs.toList
+    let φ := mkAndN eqs
+    let φ ← withLocalDeclD `tuple (mkStateTuple goal.σs) fun tuple =>
+      mkLambdaFVars #[tuple] φ
+    let φ := mkPureSPred goal.σs φ
+    let uniq ← liftMetaM <| mkFreshUserName hypName
+    let φ := Hyp.toExpr ⟨hypName, uniq, ← mkLambdaFVars ss φ⟩
+    return (← mkLambdaFVars ss H, φ)
+
+  -- Build `⟨rfl, ..., rfl⟩ : e₁ = e₁ ∧ ... ∧ eₙ = eₙ`
+  let prfs ← liftMetaM <| revertArgs.mapM mkEqRefl
+  let h ← mkAndIntroN prfs.toList
+
+  -- Push `fun s₁ ... sₙ =>` into the hyps in `H`
+  let σs' := revertArgsTypes.foldr TypeList.mkCons goal.σs
+  let H ← instantiateMVarsIfMVarApp H
+  let H := pushForallContextIntoHyps σs' H
+  let (H, hand) := mkAnd σs' H φ
+
+  -- Prove `((fun s₁ ... sₙ => H) ∧ (fun s₁ ... sₙ => ⌜s₁ = e₁ ∧ ... ∧ sₙ = eₙ⌝)) ⊢ₛ T`
+  let goal' := { σs := σs', hyps := H, target := mkAppRev f args[n:] }
+  let (a, prf) ← k goal'
+
+  -- Build the proof for `H ⊢ₛ T e₁ ... eₙ`
+  let prf := mkApp8 (mkConst ``Revert.and_pure_intro_r) goal.σs (← inferType h) goal.hyps (mkAppN H revertArgs) goal.target h (mkAppN hand revertArgs) (mkAppN prf revertArgs)
+  goal.checkProof prf
+  return (a, prf)
 
 @[builtin_tactic Lean.Parser.Tactic.mrevert]
 def elabMRevert : Tactic
-  | `(tactic| mrevert $h) => do
-  let (mvar, goal) ← mStartMVar (← getMainGoal)
+  | `(tactic| mrevert $h:ident) => do
+  let mvar ← getMainGoal
+  let some goal := parseMGoal? (← mvar.getType)
+    | throwError "Not in proof mode"
   mvar.withContext do
-
   let goals ← IO.mkRef []
-  mvar.assign (← mRevertStep goal h fun newGoal => do
+  mvar.assign (← mRevert goal h fun newGoal => do
     let m ← mkFreshExprSyntheticOpaqueMVar newGoal.toExpr
     goals.modify (m.mvarId! :: ·)
-    return m)
+    return ((), m)).snd
+  replaceMainGoal (← goals.get)
+  | `(tactic| mrevert ∀ $[$n]?) => do
+  let (mvar, goal) ← mStartMVar (← getMainGoal)
+  mvar.withContext do
+  let n := ((·.getNat) <$> n).getD 1
+  let goals ← IO.mkRef []
+  mvar.assign (← mRevertForallN goal n (← mkFreshUserName `h) fun newGoal => do
+    let m ← mkFreshExprSyntheticOpaqueMVar newGoal.toExpr
+    goals.modify (m.mvarId! :: ·)
+    return ((), m)).snd
   replaceMainGoal (← goals.get)
   | _ => throwUnsupportedSyntax
